Lectures/Week06/Sheet2.lean
@@ -10,70 +10,145 @@ import Lectures.Week06.API
 set_option autoImplicit false
 set_option tactic.hygienic false
 
-
 -- In this sheet, we are going to prove the merge lemma
 
 def Merge: List ℕ → List ℕ → List ℕ
-  | x, [] => x
-  | [], x => x
-  | x::xs, y::ys =>
-    if x ≤ y then x :: Merge xs (y::ys)
+  | xs, [] => xs
+  | [], xs => xs
+  | x :: xs, y :: ys =>
+    if x ≤ y then x :: Merge xs (y :: ys)
     else y :: Merge (x :: xs) ys
 
 -- Example: Let's prove this by recursion
-lemma merge_size_sum (l1 l2 : List ℕ) : (Merge l1 l2).length = l1.length + l2.length  := by
-match  l1, l2 with
-| x, [] => simp [Merge]
-| [], x => unfold Merge; aesop
-| x::xs, y::ys =>
-  simp +arith +decide only [List.length_cons,Merge]
-  split_ifs
-  · simp
-    apply merge_size_sum
-  · simp
-    have: xs.length + ys.length + 1 = (xs.length +1 ) + ys.length := by omega
-    rw [this]
-    apply merge_size_sum
+lemma merge_size_sum (l1 l2 : List ℕ)
+ : (Merge l1 l2).length = l1.length + l2.length  := by
+ match  l1, l2 with
+ | x, [] => simp [Merge]
+ | [], x => unfold Merge; aesop
+ | x::xs, y::ys =>
+   simp +arith +decide only [List.length_cons, Merge]
+   split_ifs
+   · simp
+     -- rw [merge_size_sum] ; rfl
+     apply merge_size_sum
+   · simp
+     have h₁ : xs.length + ys.length + 1 = (xs.length + 1) + ys.length := by omega
+     rw [h₁]
+     apply merge_size_sum
 
 -- Example: Let's prove this by induction
 example (l1 l2 : List ℕ) : (Merge l1 l2).length = l1.length + l2.length  := by
-fun_induction Merge l1 l2
-· simp
-· simp
-· simp
-  rw [ih1]
-  simp +arith
-· simp
-  rw [ih1]
-  simp +arith
+ fun_induction Merge l1 l2
+ · simp
+ · simp
+ · simp
+   try rw [ih1]
+   try simp +arith
+ · simp
+   try rw [ih1]
+   try simp +arith
 
 -- Example: Let's us leverage automation + functional induction
-example (l1 l2 : List ℕ) : (Merge l1 l2).length = l1.length + l2.length  := by
-fun_induction Merge l1 l2 <;> all_goals grind
+example (l1 l2 : List ℕ)
+  : (Merge l1 l2).length = l1.length + l2.length  := by
+  fun_induction Merge l1 l2 <;> grind
 
 -- Example: another theorem with this hammer
 theorem mem_either_merge_auto (xs ys : List ℕ) (z : ℕ)
   (hz : z ∈ Merge xs ys) : z ∈ xs ∨ z ∈ ys := by
-  fun_induction Merge <;> all_goals grind
+  fun_induction Merge ; all_goals grind
 
--- Let's break down the proof and see how to prove this by ``hand``.
--- Exercise 2.1: try to prove this using either recursion or functional induction (don't use grind on the inductive step)
+-- Let's break down the proof and see how to prove this by ``hand``. Exercise 2.1: try to prove this using either
+-- recursion or functional induction (don't use grind on the inductive step)
 theorem mem_either_merge (xs ys : List ℕ) (z : ℕ)
-  (hz : z ∈ Merge xs ys) : z ∈ xs ∨ z ∈ ys := by sorry
+  (hz : z ∈ Merge xs ys) : z ∈ xs ∨ z ∈ ys := by
+  induction xs, ys using Merge.induct with
+  | case1 as =>
+    simp [Merge] at * ; assumption
+  | case2 as =>
+    simp [Merge] at * ; assumption
+  | case3 a as b bs =>
+    simp [Merge, h] at hz
+    cases hz with
+    | inl h₁ => simp only [List.mem_cons, true_or, h₁]
+    | inr h₁ =>
+      have h₂ := ih1 h₁
+      cases h₂ with
+      | inl h₃ => simp only [List.mem_cons] ; left ; right ; assumption
+      | inr h₃ => right ; assumption
+  | case4 a as b bs =>
+    simp [Merge, h] at hz
+    cases hz with
+    | inl h₁ => right; simp only [List.mem_cons, true_or, h₁]
+    | inr h₁ =>
+      have h₂ := ih1 h₁
+      cases h₂ with
+      | inl h₃ => left ; assumption
+      | inr h₃ => right ; simp only [List.mem_cons] ; right ; assumption
+
 
 -- Exercise 2.2: use mem_either_merge to prove the following.
 #check mem_either_merge
-theorem min_all_merge (x : ℕ) (xs ys: List ℕ)
- (hxs : x.MinOfList xs) (hys : x.MinOfList ys) : x.MinOfList (Merge xs ys):= by sorry
 
--- We are ready to prove the main sorted merge.
--- discuss a proof
+theorem min_all_merge (x : ℕ) (xs ys : List ℕ)
+ (hxs : x.MinOfList xs) (hys : x.MinOfList ys)
+ : x.MinOfList (Merge xs ys):= by
+ rw [Nat.MinOfList]
+ intro y hy
+ apply mem_either_merge at hy
+ cases hy
+ . exact hxs y h
+ . exact hys y h
 
-theorem sorted_merge(l1 l2 : List ℕ)(hxs: Sorted l1) (hys: Sorted l2): Sorted (Merge l1 l2) := by sorry
+
+-- We are ready to prove the main sorted merge. discuss a proof
+
+theorem sorted_merge (l1 l2 : List ℕ) (hxs: Sorted l1) (hys: Sorted l2)
+  : Sorted (Merge l1 l2) := by
+  induction l1, l2 using Merge.induct with
+  | case1 as =>
+    simp [Merge]; assumption
+  | case2 as =>
+    simp [Merge]; assumption
+  | case3 a as b bs =>
+    simp [Merge, h]
+    apply Sorted.cons_min
+    apply min_all_merge
+    exact sorted_min hxs
+    intro y h₁
+    rw [List.mem_cons] at h₁
+    cases h₁
+    . rwa [h_1]
+    . apply sorted_min at hys
+      apply hys at h_1
+      trans b
+      repeat assumption
+    apply ih1
+    exact sorted_suffix hxs
+    assumption
+  | case4 a as b bs =>
+    simp [Merge, h]
+    apply Sorted.cons_min
+    apply min_all_merge
+    intro y h₁
+    rw [List.mem_cons] at h₁
+    cases h₁
+    . rw [h_1]
+      omega
+    . apply sorted_min at hxs
+      apply hxs at h_1
+      trans a
+      omega ; assumption
+    exact sorted_min hys
+    apply ih1
+    assumption
+    exact sorted_suffix hys
+
 
 -- c.f. with recursive proofs.
-theorem sorted_merge_rec(l1 l2 : List ℕ)(hxs: Sorted l1) (hys: Sorted l2): Sorted (Merge l1 l2) := by
-  match l1,l2 with
+theorem sorted_merge_rec (l1 l2 : List ℕ) (hxs: Sorted l1) (hys: Sorted l2)
+  : Sorted (Merge l1 l2) := by
+  match l1, l2 with
   | x, [] => simpa [Merge]
   | [],x => unfold Merge; aesop
   | x::xs, y::ys =>
@@ -85,7 +160,7 @@ theorem sorted_merge_rec(l1 l2 : List ℕ)(hxs: Sorted l1) (hys: Sorted l2): Sor
       · apply min_all_merge
         · grind
         · grind
-      · apply sorted_merge
+      · apply sorted_merge_rec
         · exact sorted_suffix hxs
         · exact hys
     · apply Sorted.cons_min
@@ -94,13 +169,49 @@ theorem sorted_merge_rec(l1 l2 : List ℕ)(hxs: Sorted l1) (hys: Sorted l2): Sor
       · apply min_all_merge
         · grind
         · grind
-      · apply sorted_merge
+      · apply sorted_merge_rec
         · exact hxs
         · exact sorted_suffix hys
 
 -- Exercise 2.3
-theorem merge_min_out (x : ℕ) (xs ys : List ℕ) (h_min_in_xs : ∀ y ∈ xs, x ≤ y)
-  : Merge (x :: ys) xs = x :: Merge ys xs := by sorry
+theorem merge_min_out (x : ℕ) (xs ys : List ℕ)
+  (h_min_in_xs : ∀ y ∈ xs, x ≤ y)
+  : Merge (x :: ys) xs = x :: Merge ys xs := by
+  fun_induction Merge
+  . simp [Merge]
+  . cases xs_1
+    . simp [Merge]
+    . specialize h_min_in_xs head
+      simp at h_min_in_xs
+      unfold Merge
+      simp [h_min_in_xs, Merge]
+  . specialize h_min_in_xs y
+    simp at h_min_in_xs
+    nth_rw 1 [Merge]
+    simp [h_min_in_xs]
+    nth_rw 1 [Merge]
+    simp [h]
+  . specialize h_min_in_xs y
+    simp at h_min_in_xs
+    conv =>
+      lhs
+      unfold Merge
+      simp [h_min_in_xs]
+      unfold Merge
+      simp [h]
 
 -- Exercise 2.4
-theorem merge_min_out_sym(x : ℕ) (xs ys : List ℕ) (h_min_in_xs : ∀ y ∈ xs, x ≤ y) (h_min_in_ys : ∀ y ∈ ys, x ≤ y) : Merge ys (x ::xs)  = x :: Merge ys xs := by sorry
+theorem merge_min_out_sym(x : ℕ) (xs ys : List ℕ)
+  (h_min_in_xs : ∀ y ∈ xs, x ≤ y) (h_min_in_ys : ∀ y ∈ ys, x ≤ y)
+  : Merge ys (x :: xs)  = x :: Merge ys xs := by
+  match ys with
+  | .nil =>
+    cases xs
+    . simp [Merge]
+    . simp [Merge]
+  | .cons a as =>
+    have h₁ := h_min_in_ys a ; simp at h₁
+    nth_rw 1 [Merge]
+    by_cases h1 : x = a
+    simp [h1]
+    sorry
